aarch64 ainvs: bare minimum triage and sorrying
Starting point for AArch64 abstract invariant proofs.

In most cases, commented out or sorried what doesn't work. In some
cases, had to tweak definitions to get through. Marked all
problem/failure areas with FIXME AARCH64.

Signed-off-by: Rafal Kolanski <rafal.kolanski@proofcraft.systems>

proof/invariant-abstract/AARCH64/ArchCSpaceInvPre_AI.thy
@@ -1,4 +1,5 @@
 (*
+ * Copyright 2022, Proofcraft Pty Ltd
  * Copyright 2020, Data61, CSIRO (ABN 41 687 119 230)
  *
  * SPDX-License-Identifier: GPL-2.0-only
@@ -13,7 +14,7 @@ imports CSpaceInvPre_AI
 begin
 
 
-context Arch begin global_naming RISCV64
+context Arch begin global_naming AARCH64
 
 lemma aobj_ref_acap_rights_update[simp]:
   "aobj_ref (acap_rights_update f x) = aobj_ref x"
@@ -32,7 +33,7 @@ definition cap_master_arch_cap :: "arch_cap \<Rightarrow> arch_cap" where
      (case acap of
            ASIDPoolCap pool asid \<Rightarrow> ASIDPoolCap pool 0
          | FrameCap ptr R sz dev _ \<Rightarrow> FrameCap ptr UNIV sz dev None
-         | PageTableCap ptr _ \<Rightarrow> PageTableCap ptr None
+         | PageTableCap pt_t ptr _ \<Rightarrow> PageTableCap pt_t ptr None
          | _ \<Rightarrow> acap)"
 
 lemma cap_master_arch_cap_eqDs1:
@@ -42,8 +43,8 @@ lemma cap_master_arch_cap_eqDs1:
   "cap_master_arch_cap cap = FrameCap ptr R sz dev map_data
      \<Longrightarrow> R = UNIV \<and> map_data = None
           \<and> (\<exists>R map_data. cap = FrameCap ptr R sz dev map_data)"
-  "cap_master_arch_cap cap = PageTableCap ptr data
-     \<Longrightarrow> data = None \<and> (\<exists>data. cap = PageTableCap ptr data)"
+  "cap_master_arch_cap cap = PageTableCap ptr pt_t data
+     \<Longrightarrow> data = None \<and> (\<exists>data. cap = PageTableCap ptr pt_t data)"
   by (clarsimp simp: cap_master_arch_cap_def split: arch_cap.split_asm)+
 
 lemma cap_master_arch_inv[simp]:
@@ -76,7 +77,7 @@ where
     \<comment> \<open> Don't introduce non-empty unmapped table objects. \<close>
   \<and> (is_pt_cap newcap
       \<longrightarrow> cap_asid newcap = None
-      \<longrightarrow> (\<forall>r \<in> obj_refs newcap. pts_of s r = Some empty_pt))
+      \<longrightarrow> (\<forall>r \<in> obj_refs newcap. pts_of s r = Some (empty_pt undefined)))
     \<comment> \<open> If newcap is vspace table cap such that either:
          - newcap and cap have different types or different obj_refs, or
          - newcap is unmapped while cap is mapped, \<close>
@@ -91,7 +92,7 @@ where
                      \<and> is_pt_cap cap'
                      \<and> (cap_asid newcap = None \<or> cap_asid cap' = None)) sl' s \<longrightarrow> sl' = sl))
   \<comment> \<open>Don't replace with an ASID pool. \<close>
-  \<and> \<not>is_ap_cap newcap"
+  \<and> \<not>is_ap_cap newcap" (* FIXME AARCH64: undefined in def *)
 
 definition
   replaceable_non_final_arch_cap :: "'z::state_ext state \<Rightarrow> cslot_ptr \<Rightarrow> cap \<Rightarrow> cap \<Rightarrow> bool"
@@ -137,6 +138,7 @@ lemma set_cap_valid_vs_lookup:
      set_cap cap ptr
    \<lbrace>\<lambda>rv. valid_vs_lookup\<rbrace>"
   supply split_paired_All[simp del] split_paired_Ex[simp del]
+  sorry (* FIXME AARCH64
   apply (wpsimp wp: hoare_vcg_all_lift hoare_convert_imp vs_lookup_target_lift hoare_vcg_disj_lift
               simp: valid_vs_lookup_def)
   apply (drule vs_lookup_target_level)
@@ -167,8 +169,9 @@ lemma set_cap_valid_vs_lookup:
    apply (erule_tac x=level in allE)
    apply (clarsimp)
   apply fastforce
-  done
+  done *)
 
+(* FIXME AARCH64
 lemma set_cap_valid_table_caps:
   "\<lbrace>\<lambda>s. valid_table_caps s \<and>
         (is_pt_cap cap \<longrightarrow> cap_asid cap = None \<longrightarrow> (\<forall>r \<in> obj_refs cap. pts_of s r = Some empty_pt))\<rbrace>
@@ -180,7 +183,7 @@ lemma set_cap_valid_table_caps:
             hoare_vcg_disj_lift hoare_convert_imp[OF set_cap_caps_of_state]
             hoare_use_eq[OF set_cap_arch set_cap_obj_at_impossible])
   apply (fastforce simp: cap_asid_def split: if_split_asm)
-  done
+  done *)
 
 lemma cap_asid_vs_cap_ref_None:
   "is_pt_cap cap \<Longrightarrow> (cap_asid cap = None) = (vs_cap_ref cap = None)"
@@ -295,7 +298,7 @@ lemma set_cap_valid_arch_caps:
                  \<or> (\<forall>oref \<in> obj_refs cap'. \<not> reachable_target vref oref s))
       \<and> no_cap_to_obj_with_diff_ref cap {ptr} s
       \<and> (is_pt_cap cap \<longrightarrow> cap_asid cap = None
-            \<longrightarrow> (\<forall>r \<in> obj_refs cap. pts_of s r = Some empty_pt))
+            \<longrightarrow> (\<forall>r \<in> obj_refs cap. pts_of s r = Some (empty_pt FIXME)))
       \<and> (is_pt_cap cap
              \<longrightarrow> (\<forall>oldcap. caps_of_state s ptr = Some oldcap \<longrightarrow>
                   is_pt_cap oldcap
@@ -307,9 +310,11 @@ lemma set_cap_valid_arch_caps:
      set_cap cap ptr
    \<lbrace>\<lambda>rv. valid_arch_caps\<rbrace>"
   unfolding valid_arch_caps_def
+  sorry (*
   by (wpsimp wp: set_cap_valid_vs_lookup set_cap_valid_table_caps set_cap_unique_table_caps
-           simp: cte_wp_at_caps_of_state)
+           simp: cte_wp_at_caps_of_state) *)
 
+(* FIXME AARCH64
 lemma valid_table_capsD:
   "\<lbrakk> cte_wp_at ((=) cap) ptr s; valid_table_caps s; is_pt_cap cap; cap_asid cap = None \<rbrakk>
    \<Longrightarrow> \<forall>r \<in> obj_refs cap. pts_of s r = Some empty_pt"
@@ -317,7 +322,7 @@ lemma valid_table_capsD:
                         is_PageTableCap_def cap_asid_def
                  split: option.splits)
    apply (cases ptr, fastforce)+
-  done
+  done *)
 
 lemma pt_caps_asid_vsref:
   "is_pt_cap cap \<Longrightarrow> (cap_asid cap = None) = (vs_cap_ref cap = None)"
